\documentclass{article}
\usepackage{amsmath}
\begin{document}
\newcommand{\softmax}[2]{ [softmax(#1)]_{#2} }
\begin{multline}
J_{jk} = \frac{\partial \softmax{z}{j}}{\partial z_{k}} =
\frac{\partial}{\partial z_{k}} \frac{exp(z_{j})}{\sum_{i=1}^{K} exp(z_{i})} =
\left\{
\begin{array}{ll}
	-\frac{exp(z_{j}) exp(z_{k})}{\left[ \sum_{i=1}^{K} exp(z_{i}) \right]^{2}}, & j \neq k \\
	\frac{\partial}{\partial z_{j}} \frac{exp(z_{j})}{\sum_{i=1}^{K} exp(z_{i})}, & j = k
\end{array}
\right.
\\ =
\left\{
\begin{array}{ll}
	- \softmax{z}{j} \softmax{z}{k}, & j \neq k \\
	\softmax{z}{j} (1 - \softmax{z}{j}), & j = k
\end{array}
\right.
\end{multline}

\newcommand{\sumezi}{\left(\sum_{i=1}^{K} exp(z_{i}) \right)}
\begin{equation}
\begin{split}
	\frac{\partial}{\partial z_{j}} \frac{exp(z_{j})}{\sum_{i=1}^{K} exp(z_{i})} = \\
=
\frac
	{\left( \frac{\partial}{\partial z_{j}} exp(z_{j}) \right) \sumezi - exp(z_{j}) \frac{\partial}{\partial z_{j}} \sumezi}
	{\sumezi^{2}} = \\
=
\frac
	{exp(z_{j}) \left(\sumezi - exp(2z_j) \right)}
	{ \sumezi ^{2}} = \\
\frac
	{exp(z_{j}) \left(\sumezi - exp(z_j) \right)}
	{\sumezi ^{2}} = \\
\frac
	{\softmax{z}{j} \left(\sumezi - exp(z_{j}) \right)}
	{\sumezi} = \\
\softmax{z}{j} (1 - \softmax{z}{j})
\end{split}
\end{equation}
\end{document}
